nola/iris/inv_deriv.v
@@ -21,16 +21,16 @@ Arguments INV_PRE_DERIV {_ _} _ {_}.
 
 Section inv_deriv.
   Context `{!InvPreDeriv FM JUDG} {Σ : gFunctors}.
-  Implicit Type δ : JUDG → iProp Σ.
+  Implicit Type (δ : JUDG → iProp Σ) (Px : FM).
 
   (** [inv']: Relaxed invariant *)
-  Local Definition inv'_def δ N (P : FM) : iProp Σ := □ δ (inv_jacsr N P).
+  Local Definition inv'_def δ N Px : iProp Σ := □ δ (inv_jacsr N Px).
   Local Lemma inv'_aux : seal inv'_def. Proof. by eexists. Qed.
   Definition inv' := inv'_aux.(unseal).
   Local Lemma inv'_unseal : inv' = inv'_def. Proof. exact: seal_eq. Qed.
 
   (** [inv'] is persistent *)
-  #[export] Instance inv'_persistent {δ N P} : Persistent (inv' δ N P).
+  #[export] Instance inv'_persistent {δ N Px} : Persistent (inv' δ N Px).
   Proof. rewrite inv'_unseal. exact _. Qed.
 
   (** [inv'] is non-expansive *)
@@ -41,7 +41,7 @@ Notation invd := (inv' der).
 
 Section inv_deriv.
   Context `{!inv'GS FML Σ, !invGS_gen hlc Σ}.
-  Implicit Type P Q PQ : FML $oi Σ.
+  Implicit Type Px Qx PQx : FML $oi Σ.
 
   (** Accessor to the invariant body *)
   Definition inv_acsr sm N Pi : iProp Σ :=
@@ -55,99 +55,101 @@ Section inv_deriv.
   (** Derivability data for [inv] *)
   Class InvDeriv :=
     (** Interpreting [inv_jacsr] *)
-    inv_jacsr_sem : ∀{δ N P},
-      ⟦ inv_jacsr N P ⟧(δ) ⊣⊢ inv_acsr ⟦⟧(δ) N ⟦ P ⟧(δ).
+    inv_jacsr_sem : ∀{δ N Px},
+      ⟦ inv_jacsr N Px ⟧(δ) ⊣⊢ inv_acsr ⟦⟧(δ) N ⟦ Px ⟧(δ).
 
   Context `{!InvDeriv}.
 
   (** Access [inv'] *)
-  Lemma invd_acc {N P E} : ↑N ⊆ E →
-    invd N P =[inv_wsatid]{E,E∖↑N}=∗
-      ⟦ P ⟧ ∗ (⟦ P ⟧ =[inv_wsatid]{E∖↑N,E}=∗ True).
+  Lemma invd_acc {N Px E} : ↑N ⊆ E →
+    invd N Px =[inv_wsatid]{E,E∖↑N}=∗
+      ⟦ Px ⟧ ∗ (⟦ Px ⟧ =[inv_wsatid]{E∖↑N,E}=∗ True).
   Proof.
-    rewrite inv'_unseal. iIntros (?) "accP".
-    iDestruct (der_sound with "accP") as "accP". rewrite inv_jacsr_sem.
-    by iApply "accP".
+    rewrite inv'_unseal. iIntros (?) "accPx".
+    iDestruct (der_sound with "accPx") as "accPx". rewrite inv_jacsr_sem.
+    by iApply "accPx".
   Qed.
 
   Context `{!Deriv (JUDGI:=JUDGI) ih δ}.
 
   (** Turn [inv_acsr] into [inv'] *)
-  Lemma inv_acsr_inv' {N P} :
+  Lemma inv_acsr_inv' {N Px} :
     □ (∀ δ', ⌜Deriv ih δ'⌝ → ⌜ih δ'⌝ → ⌜dinto δ δ'⌝ →
-      inv_acsr ⟦⟧(δ') N ⟦ P ⟧(δ')) ⊢ inv' δ N P.
+      inv_acsr ⟦⟧(δ') N ⟦ Px ⟧(δ')) ⊢ inv' δ N Px.
   Proof.
     rewrite inv'_unseal. iIntros "#big !>". iApply Deriv_factor. iIntros (????).
     rewrite inv_jacsr_sem. by iApply "big".
   Qed.
 
   (** Turn [inv_tok] into [inv'] *)
-  Lemma inv_tok_inv' {N P} : inv_tok N P ⊢ inv' δ N P.
+  Lemma inv_tok_inv' {N Px} : inv_tok N Px ⊢ inv' δ N Px.
   Proof.
     rewrite -inv_acsr_inv'. iIntros "#i !>" (δ' ?????).
     by iApply (inv_tok_acc (sm:=⟦⟧(δ')) with "i").
   Qed.
 
   (** Allocate [inv'] *)
-  Lemma inv'_alloc_rec P N :
-    (inv' δ N P -∗ ⟦ P ⟧(δ)) =[inv_wsati δ]=∗ inv' δ N P.
+  Lemma inv'_alloc_rec Px N :
+    (inv' δ N Px -∗ ⟦ Px ⟧(δ)) =[inv_wsati δ]=∗ inv' δ N Px.
   Proof. rewrite -inv_tok_inv'. exact: inv_tok_alloc_rec. Qed.
-  Lemma inv'_alloc P N : ⟦ P ⟧(δ) =[inv_wsati δ]=∗ inv' δ N P.
+  Lemma inv'_alloc Px N : ⟦ Px ⟧(δ) =[inv_wsati δ]=∗ inv' δ N Px.
   Proof. rewrite -inv_tok_inv'. exact: inv_tok_alloc. Qed.
-  Lemma inv'_alloc_open P N E : ↑N ⊆ E →
-    ⊢ |=[inv_wsati δ]{E, E∖↑N}=> inv' δ N P ∗
-      (⟦ P ⟧(δ) =[inv_wsati δ]{E∖↑N, E}=∗ True).
+  Lemma inv'_alloc_open Px N E : ↑N ⊆ E →
+    ⊢ |=[inv_wsati δ]{E, E∖↑N}=> inv' δ N Px ∗
+      (⟦ Px ⟧(δ) =[inv_wsati δ]{E∖↑N, E}=∗ True).
   Proof. rewrite -inv_tok_inv'. exact: inv_tok_alloc_open. Qed.
 
   (** Convert [inv'] with [mod_acsr] *)
-  Lemma inv'_acsr {N P Q} :
+  Lemma inv'_acsr {N Px Qx} :
     □ (∀ δ', ⌜Deriv ih δ'⌝ → ⌜ih δ'⌝ → ⌜dinto δ δ'⌝ →
-      mod_acsr (fupd ∅ ∅) ⟦ P ⟧(δ') ⟦ Q ⟧(δ')) -∗
-      inv' δ N P -∗ inv' δ N Q.
+      mod_acsr (fupd ∅ ∅) ⟦ Px ⟧(δ') ⟦ Qx ⟧(δ')) -∗
+      inv' δ N Px -∗ inv' δ N Qx.
   Proof.
-    rewrite inv'_unseal. iIntros "#PQP #accP !>". iApply Deriv_factor.
+    rewrite inv'_unseal. iIntros "#PQP #accPx !>". iApply Deriv_factor.
     iIntros (??? to). rewrite to !inv_jacsr_sem. iIntros (? NE).
-    iMod ("accP" $! _ NE) as "[P cl]".
+    iMod ("accPx" $! _ NE) as "[Px cl]".
     iMod (fupd_mask_subseteq ∅) as "→E∖N"; [set_solver|].
-    iMod ("PQP" with "[//] [//] [//] P") as "($& QP)". iMod "→E∖N" as "_".
-    iIntros "!> Q". iMod (fupd_mask_subseteq ∅) as "→E∖N"; [set_solver|].
-    iMod ("QP" with "Q") as "P". iMod "→E∖N" as "_". iApply ("cl" with "P").
+    iMod ("PQP" with "[//] [//] [//] Px") as "($& QP)". iMod "→E∖N" as "_".
+    iIntros "!> Qx". iMod (fupd_mask_subseteq ∅) as "→E∖N"; [set_solver|].
+    iMod ("QP" with "Qx") as "Px". iMod "→E∖N" as "_". iApply ("cl" with "Px").
   Qed.
-  Lemma inv'_iff {N P Q} :
+  Lemma inv'_iff {N Px Qx} :
     □ (∀ δ', ⌜Deriv ih δ'⌝ → ⌜ih δ'⌝ → ⌜dinto δ δ'⌝ →
-      ⟦ P ⟧(δ') ∗-∗ ⟦ Q ⟧(δ')) -∗
-      inv' δ N P -∗ inv' δ N Q.
+      ⟦ Px ⟧(δ') ∗-∗ ⟦ Qx ⟧(δ')) -∗
+      inv' δ N Px -∗ inv' δ N Qx.
   Proof.
     iIntros "#big". iApply inv'_acsr. iIntros "!>" (????).
     iApply (wand_iff_mod_acsr (M:=fupd _ _)). iModIntro. by iApply "big".
   Qed.
 
   (** Split [inv'] over [∗] *)
-  Local Lemma inv'_sep' {N PQ P Q} :
-    (∀ δ', ⟦ PQ ⟧(δ') ≡ (⟦ P ⟧(δ') ∗ ⟦ Q ⟧(δ'))%I) → inv' δ N PQ ⊢ inv' δ N P.
+  Local Lemma inv'_sep' {N PQx Px Qx} :
+    (∀ δ', ⟦ PQx ⟧(δ') ≡ (⟦ Px ⟧(δ') ∗ ⟦ Qx ⟧(δ'))%I) →
+    inv' δ N PQx ⊢ inv' δ N Px.
   Proof.
     iIntros (eq). iApply (inv'_acsr with "[]"). iIntros "!>" (????).
     rewrite eq. iApply (mod_acsr_sep_l (M:=fupd _ _)).
   Qed.
-  Lemma inv'_sep {N PQ P Q} : (∀ δ', ⟦ PQ ⟧(δ') ≡ (⟦ P ⟧(δ') ∗ ⟦ Q ⟧(δ'))%I) →
-    inv' δ N PQ ⊢ inv' δ N P ∗ inv' δ N Q.
+  Lemma inv'_sep {N PQx Px Qx} :
+    (∀ δ', ⟦ PQx ⟧(δ') ≡ (⟦ Px ⟧(δ') ∗ ⟦ Qx ⟧(δ'))%I) →
+    inv' δ N PQx ⊢ inv' δ N Px ∗ inv' δ N Qx.
   Proof.
     iIntros (eq) "#i". iSplit; [by iApply inv'_sep'|].
     iApply (inv'_sep' with "i"). iIntros (?). by rewrite eq comm.
   Qed.
 
   (** Merge [inv']s with [∗] *)
-  Lemma inv'_merge {N1 N2 N P Q PQ} : N1 ## N2 → ↑N1 ∪ ↑N2 ⊆@{coPset} ↑N →
-    (∀ δ', ⟦ PQ ⟧(δ') ≡ (⟦ P ⟧(δ') ∗ ⟦ Q ⟧(δ'))%I) →
-    inv' δ N1 P -∗ inv' δ N2 Q -∗ inv' δ N PQ.
+  Lemma inv'_merge {N1 N2 N Px Qx PQx} : N1 ## N2 → ↑N1 ∪ ↑N2 ⊆@{coPset} ↑N →
+    (∀ δ', ⟦ PQx ⟧(δ') ≡ (⟦ Px ⟧(δ') ∗ ⟦ Qx ⟧(δ'))%I) →
+    inv' δ N1 Px -∗ inv' δ N2 Qx -∗ inv' δ N PQx.
   Proof.
     rewrite inv'_unseal. iIntros (?? eq) "#i #i' !>".
     iApply (Deriv_map2 with "[] i i'"). iIntros (????) "{i}i {i'}i'".
     rewrite !inv_jacsr_sem. iIntros (??). rewrite eq.
-    iMod ("i" with "[%]") as "[$ P→]"; [set_solver|].
-    iMod ("i'" with "[%]") as "[$ Q→]"; [set_solver|].
-    iApply fupdw_mask_intro; [set_solver|]. iIntros "cl [P Q]".
-    iMod "cl" as "_". iMod ("Q→" with "Q") as "_". iApply ("P→" with "P").
+    iMod ("i" with "[%]") as "[$ Px→]"; [set_solver|].
+    iMod ("i'" with "[%]") as "[$ Qx→]"; [set_solver|].
+    iApply fupdw_mask_intro; [set_solver|]. iIntros "cl [Px Qx]".
+    iMod "cl" as "_". iMod ("Qx→" with "Qx") as "_". iApply ("Px→" with "Px").
   Qed.
 End inv_deriv.
 Arguments InvDeriv FML Σ {_ _ _} JUDGI {_ _}.
