nola/iris/na_inv_deriv.v
@@ -24,16 +24,16 @@ Section na_inv_deriv.
   Implicit Type δ : JUDG → iProp Σ.
 
   (** [na_inv']: Relaxed na_invariant *)
-  Local Definition na_inv'_def δ p N (P : FM) : iProp Σ :=
-    □ δ (na_inv_jacsr p N P).
+  Local Definition na_inv'_def δ p N (Px : FM) : iProp Σ :=
+    □ δ (na_inv_jacsr p N Px).
   Local Lemma na_inv'_aux : seal na_inv'_def. Proof. by eexists. Qed.
   Definition na_inv' := na_inv'_aux.(unseal).
   Local Lemma na_inv'_unseal : na_inv' = na_inv'_def.
   Proof. exact: seal_eq. Qed.
 
   (** [na_inv'] is persistent *)
-  #[export] Instance na_inv'_persistent {δ p N P} :
-    Persistent (na_inv' δ p N P).
+  #[export] Instance na_inv'_persistent {δ p N Px} :
+    Persistent (na_inv' δ p N Px).
   Proof. rewrite na_inv'_unseal. exact _. Qed.
 
   (** [na_inv'] is non-expansive *)
@@ -45,7 +45,7 @@ Notation na_invd := (na_inv' der).
 
 Section na_inv_deriv.
   Context `{!na_inv'GS FML Σ, !invGS_gen hlc Σ, !na_invG Σ}.
-  Implicit Type P Q PQ : FML $oi Σ.
+  Implicit Type Px Qx PQx : FML $oi Σ.
 
   (** Accessor *)
   Definition na_inv_acsr sm p N Pi : iProp Σ :=
@@ -60,16 +60,16 @@ Section na_inv_deriv.
   (** Derivability data for [na_inv] *)
   Class NaInvDeriv :=
     (** Interpreting [na_inv_jacsr] *)
-    na_inv_jacsr_sem : ∀{δ p N P},
-      ⟦ na_inv_jacsr p N P ⟧(δ) ⊣⊢ na_inv_acsr ⟦⟧(δ) p N (⟦ P ⟧(δ)).
+    na_inv_jacsr_sem : ∀{δ p N Px},
+      ⟦ na_inv_jacsr p N Px ⟧(δ) ⊣⊢ na_inv_acsr ⟦⟧(δ) p N (⟦ Px ⟧(δ)).
 
   Context `{!NaInvDeriv}.
 
   (** Access [na_invd] *)
-  Lemma na_invd_acc {p N P E F} : ↑N ⊆ E → ↑N ⊆ F →
-    na_own p F -∗ na_invd p N P =[na_inv_wsatid]{E}=∗
-      na_own p (F∖↑N) ∗ ⟦ P ⟧ ∗
-      (na_own p (F∖↑N) -∗ ⟦ P ⟧ =[na_inv_wsatid]{E}=∗ na_own p F).
+  Lemma na_invd_acc {p N Px E F} : ↑N ⊆ E → ↑N ⊆ F →
+    na_own p F -∗ na_invd p N Px =[na_inv_wsatid]{E}=∗
+      na_own p (F∖↑N) ∗ ⟦ Px ⟧ ∗
+      (na_own p (F∖↑N) -∗ ⟦ Px ⟧ =[na_inv_wsatid]{E}=∗ na_own p F).
   Proof.
     rewrite na_inv'_unseal. iIntros (NE NF) "F accP".
     iDestruct (der_sound with "accP") as "accP". rewrite na_inv_jacsr_sem.
@@ -79,78 +79,79 @@ Section na_inv_deriv.
   Context `{!Deriv (JUDGI:=JUDGI) ih δ}.
 
   (** Turn [na_inv_acsr] into [na_inv'] *)
-  Lemma na_inv_acsr_inv' {p N P} :
+  Lemma na_inv_acsr_inv' {p N Px} :
     □ (∀ δ', ⌜Deriv ih δ'⌝ → ⌜ih δ'⌝ → ⌜dinto δ δ'⌝ →
-      na_inv_acsr ⟦⟧(δ') p N ⟦ P ⟧(δ')) ⊢ na_inv' δ p N P.
+      na_inv_acsr ⟦⟧(δ') p N ⟦ Px ⟧(δ')) ⊢ na_inv' δ p N Px.
   Proof.
     rewrite na_inv'_unseal. iIntros "#big !>". iApply Deriv_factor.
     iIntros (????). rewrite na_inv_jacsr_sem. by iApply "big".
   Qed.
 
   (** Turn [na_inv_tok] into [na_inv'] *)
-  Lemma na_inv_tok_na_inv' {p N P} : na_inv_tok p N P ⊢ na_inv' δ p N P.
+  Lemma na_inv_tok_na_inv' {p N Px} : na_inv_tok p N Px ⊢ na_inv' δ p N Px.
   Proof.
     rewrite -na_inv_acsr_inv'. iIntros "#i !>" (δ' ???????) "F".
     by iApply (na_inv_tok_acc (sm:=⟦⟧(δ')) with "F i").
   Qed.
 
   (** Allocate [na_inv'] *)
-  Lemma na_inv'_alloc_rec p P N :
-    (na_inv' δ p N P -∗ ⟦ P ⟧(δ)) =[na_inv_wsati δ]=∗ na_inv' δ p N P.
+  Lemma na_inv'_alloc_rec p Px N :
+    (na_inv' δ p N Px -∗ ⟦ Px ⟧(δ)) =[na_inv_wsati δ]=∗ na_inv' δ p N Px.
   Proof. rewrite -na_inv_tok_na_inv'. exact: na_inv_tok_alloc_rec. Qed.
-  Lemma na_inv'_alloc p P N : ⟦ P ⟧(δ) =[na_inv_wsati δ]=∗ na_inv' δ p N P.
+  Lemma na_inv'_alloc p Px N : ⟦ Px ⟧(δ) =[na_inv_wsati δ]=∗ na_inv' δ p N Px.
   Proof. rewrite -na_inv_tok_na_inv'. exact: na_inv_tok_alloc. Qed.
-  Lemma na_inv'_alloc_open p N E F P :
+  Lemma na_inv'_alloc_open p N E F Px :
     ↑N ⊆ E → ↑N ⊆ F →
     na_own p F =[na_inv_wsati δ]{E}=∗
-      na_own p (F∖↑N) ∗ na_inv' δ p N P ∗
-      (na_own p (F∖↑N) -∗ ⟦ P ⟧(δ) =[na_inv_wsati δ]{E}=∗ na_own p F).
+      na_own p (F∖↑N) ∗ na_inv' δ p N Px ∗
+      (na_own p (F∖↑N) -∗ ⟦ Px ⟧(δ) =[na_inv_wsati δ]{E}=∗ na_own p F).
   Proof. rewrite -na_inv_tok_na_inv'. exact: na_inv_tok_alloc_open. Qed.
 
   (** Convert [na_inv'] with [mod_acsr] *)
-  Lemma na_inv'_acsr {p N P Q} :
+  Lemma na_inv'_acsr {p N Px Qx} :
     □ (∀ δ', ⌜Deriv ih δ'⌝ → ⌜ih δ'⌝ → ⌜dinto δ δ'⌝ →
-      mod_acsr (fupd ∅ ∅) ⟦ P ⟧(δ') ⟦ Q ⟧(δ')) -∗
-      na_inv' δ p N P -∗ na_inv' δ p N Q.
+      mod_acsr (fupd ∅ ∅) ⟦ Px ⟧(δ') ⟦ Qx ⟧(δ')) -∗
+      na_inv' δ p N Px -∗ na_inv' δ p N Qx.
   Proof.
     rewrite na_inv'_unseal. iIntros "#PQP #accP !>". iApply Deriv_factor.
     iIntros (??? to). rewrite to !na_inv_jacsr_sem. iIntros (?? NE NF) "F".
-    iMod ("accP" $! _ _ NE NF with "F") as "($ & P & cl)".
+    iMod ("accP" $! _ _ NE NF with "F") as "($ & Px & cl)".
     iMod (fupd_mask_subseteq ∅) as "→E∖N"; [set_solver|].
-    iMod ("PQP" with "[//] [//] [//] P") as "[$ QP]". iMod "→E∖N" as "_".
+    iMod ("PQP" with "[//] [//] [//] Px") as "[$ QP]". iMod "→E∖N" as "_".
     iIntros "!>". iMod (fupd_mask_subseteq ∅) as "→E∖N"; [set_solver|].
-    iIntros "F∖N Q". iMod ("QP" with "Q") as "P". iMod "→E∖N" as "_".
-    iApply ("cl" with "F∖N P").
+    iIntros "F∖N Qx". iMod ("QP" with "Qx") as "Px". iMod "→E∖N" as "_".
+    iApply ("cl" with "F∖N Px").
   Qed.
-  Lemma na_inv'_iff {p N P Q} :
+  Lemma na_inv'_iff {p N Px Qx} :
     □ (∀ δ', ⌜Deriv ih δ'⌝ → ⌜ih δ'⌝ → ⌜dinto δ δ'⌝ →
-      ⟦ P ⟧(δ') ∗-∗ ⟦ Q ⟧(δ')) -∗
-      na_inv' δ p N P -∗ na_inv' δ p N Q.
+      ⟦ Px ⟧(δ') ∗-∗ ⟦ Qx ⟧(δ')) -∗
+      na_inv' δ p N Px -∗ na_inv' δ p N Qx.
   Proof.
     iIntros "#big". iApply na_inv'_acsr. iIntros "!>" (????).
     iApply (wand_iff_mod_acsr (M:=fupd _ _)). iModIntro. by iApply "big".
   Qed.
 
   (** Split [na_inv'] over [∗] *)
-  Local Lemma na_inv'_sep' {p N PQ P Q} :
-    (∀ δ', ⟦ PQ ⟧(δ') ≡ (⟦ P ⟧(δ') ∗ ⟦ Q ⟧(δ'))%I) →
-    na_inv' δ p N PQ ⊢ na_inv' δ p N P.
+  Local Lemma na_inv'_sep' {p N PQx Px Qx} :
+    (∀ δ', ⟦ PQx ⟧(δ') ≡ (⟦ Px ⟧(δ') ∗ ⟦ Qx ⟧(δ'))%I) →
+    na_inv' δ p N PQx ⊢ na_inv' δ p N Px.
   Proof.
     iIntros (eq). iApply (na_inv'_acsr with "[]"). iIntros "!>" (????).
     rewrite eq. iApply (mod_acsr_sep_l (M:=fupd _ _)).
   Qed.
-  Lemma na_inv'_sep {p N PQ P Q} :
-    (∀ δ', ⟦ PQ ⟧(δ') ≡ (⟦ P ⟧(δ') ∗ ⟦ Q ⟧(δ'))%I) →
-    na_inv' δ p N PQ ⊢ na_inv' δ p N P ∗ na_inv' δ p N Q.
+  Lemma na_inv'_sep {p N PQx Px Qx} :
+    (∀ δ', ⟦ PQx ⟧(δ') ≡ (⟦ Px ⟧(δ') ∗ ⟦ Qx ⟧(δ'))%I) →
+    na_inv' δ p N PQx ⊢ na_inv' δ p N Px ∗ na_inv' δ p N Qx.
   Proof.
     iIntros (eq) "#i". iSplit; [by iApply na_inv'_sep'|].
     iApply (na_inv'_sep' with "i"). iIntros (?). by rewrite eq comm.
   Qed.
 
   (** Merge [na_inv']s with [∗] *)
-  Lemma na_inv'_merge {p N1 N2 N P Q PQ} : N1 ## N2 → ↑N1 ∪ ↑N2 ⊆@{coPset} ↑N →
-    (∀ δ', ⟦ PQ ⟧(δ') ≡ (⟦ P ⟧(δ') ∗ ⟦ Q ⟧(δ'))%I) →
-    na_inv' δ p N1 P -∗ na_inv' δ p N2 Q -∗ na_inv' δ p N PQ.
+  Lemma na_inv'_merge {p N1 N2 N Px Qx PQx} :
+    N1 ## N2 → ↑N1 ∪ ↑N2 ⊆@{coPset} ↑N →
+    (∀ δ', ⟦ PQx ⟧(δ') ≡ (⟦ Px ⟧(δ') ∗ ⟦ Qx ⟧(δ'))%I) →
+    na_inv' δ p N1 Px -∗ na_inv' δ p N2 Qx -∗ na_inv' δ p N PQx.
   Proof.
     rewrite na_inv'_unseal. iIntros (?? eq) "#i #i' !>".
     iApply (Deriv_map2 with "[] i i'"). iIntros (????) "{i}i {i'}i'".
@@ -158,9 +159,9 @@ Section na_inv_deriv.
     iMod ("i" with "[%] [%] F") as "(F∖N1 & $ & P→)"; [set_solver..|].
     iMod ("i'" with "[%] [%] F∖N1") as "(F∖N12 & $ & Q→)"; [set_solver..|].
     iDestruct (na_own_acc with "F∖N12") as "[$ F∖N→]"; [set_solver|].
-    iApply fupdw_mask_intro; [set_solver|]. iIntros "cl F∖N [P Q]".
+    iApply fupdw_mask_intro; [set_solver|]. iIntros "cl F∖N [Px Qx]".
     iMod "cl" as "_". iDestruct ("F∖N→" with "F∖N") as "F∖N12".
-    iMod ("Q→" with "F∖N12 Q") as "F∖N". iApply ("P→" with "F∖N P").
+    iMod ("Q→" with "F∖N12 Qx") as "F∖N". iApply ("P→" with "F∖N Px").
   Qed.
 End na_inv_deriv.
 Arguments NaInvDeriv FML Σ {_ _ _ _} JUDGI {_ _}.
